\ssc{David's note: Determining noise from deterministic forces}
\textit{Here is the note of David Dean, considering the Brownian motion but only in two dimension ($\Delta, X$). The rotation had been neglected ($\dot\Theta=0$), and the second derivatives in the first-order correction of $\kappa$ as well. To be clear, Fokker-Planck equation would be carefully discussed. Other personal comments are also written in Italic.}

Consider the following deterministic equations \tit{($\alpha$ refers to $\Delta, X$ these two directions)}
\beq dX_\alpha = V_\alpha dt \tag{David.1} \label{David.1} \eeq
and \tit{($\mathbf{X},\mathbf{V}$ refer to the position and the velocity, respectively)}
\beq dV_\alpha = -U_\alpha dt - \nabla \phi(\mathbf{X}) dt \tlag{David.2} \eeq 
We assume that $U_\alpha$ are generated by hydrodynamic interactions which do not however affect the equilibrium Gibbs-Boltzmann distribution which is \beq P_{eq} (\mathbf{X},\mathbf{V}) = \frac{1}{\bar{Z}} \exp \left( - \frac{\beta \mathbf{V}^2}{2} - \beta \phi(\mathbf{X}) \right) \tlag{David.3} \eeq

\textit{Exploit the Fokker-Planck operator ($\cdots$ refers the similar terms about $X_\alpha$)}
$$ \pder[P]{t} = - H_{FP} P = \pder{x} \left[ \frac{dV}{dx} P + T \pder{x} P \right] = \pder{V_\alpha} \left[ (U_\alpha + \nabla_\alpha \phi) P + T \gamma_{\alpha\beta} \pder[P]{V_\beta} \right] + \pder{X_\alpha} \left[ \cdots \right] $$
\tit{Note $\pder[P]{X_\alpha} = P \left( -\beta \pder[\phi]{X_\alpha} \right)$ and $\pder[P]{V_\alpha} = P \left( -\beta V_\alpha \right)$. Consider the gravity $\phi(\mathbf{X}) = - mg\Delta$, and then we could derive the eq. \ref{David.4}, regarding $k_B$ as 1}
$$ \bgn
\pder{X_\alpha} \left[ \frac{dV}{dx} P + T \pder{x} P \right] &= \pder{X_\alpha} \left[ \frac{dV}{dX_\alpha} P + T \pder{X_\alpha} P + T \pder{V_\alpha} P \right] \\
&= \pder{X_\alpha} \left[ (\nabla_\alpha\phi)P + \cancel{T} \cdot P \left( -\cancel{\beta} \pder[\phi]{X_\alpha} \right) + T \pder{V_\alpha} P \right] = \pder{X_\alpha} \left[ T \pder{V_\alpha} P \right] \\
&= \pder{X_\alpha} \left[ \cancel{T} \cdot P \left( -\cancel\beta V_\alpha \right) \right] = - \pder{X_\alpha} V_\alpha P
\end{align} $$

The Fokker Planck equation at finite temperature which introduces white noise and possibly temperature dependent drifts is $\phi(\mathbf{X})$ is 
\beq \pder[P]{t} = \pder{V_\alpha} \left[ T \gamma_{\alpha\beta} \pder[P]{V_\beta} + U_\alpha P + \pder[\phi]{X_\alpha} P \right] - \pder{X_\alpha} V_\alpha P  \tlag{David.4} \eeq
\tit{The last two terms would vanish since}
$$ \pder{V_\alpha} \left( \pder[\phi]{X_\alpha} P \right) = \cancel{ \left( \pder{V_\alpha} \pder[\phi]{X_\alpha} \right) } \cdot P + \pder[\phi]{X_\alpha} \cdot \pder[P]{V_\alpha} = \pder[\phi]{X_\alpha} \cdot P (-\beta V_\alpha) $$
$$ \pder{X_\alpha} V_\alpha P = \cancel{ \left( \pder[V_\alpha]{X_\alpha} \right) } P + V_\alpha \left( \pder[P]{X_\alpha} \right) = V_\alpha \cdot P \cdot \left( -\beta \pder[\phi]{X_\alpha} \right) $$
\tit{Therefore, at equilibrium $\pder[P]{t} = 0$}
$$ \pder[P]{t} = \pder{V_\alpha} \left[ T \gamma_{\alpha\beta} \pder[P]{V_\beta} + U_\alpha P \right] = \pder{V_\alpha} \left[ \cancel{T} \gamma_{\alpha\beta} P \cdot (- \cancel\beta V_\beta) + U_\alpha P \right] = \pder{V_\alpha} \left[ (U_\alpha - \gamma_{\alpha\beta} V_\beta) \cdot P \right] = 0 $$

We obtain the GB distribution for the steady state if 
\beq U_\alpha = \gamma_{\alpha\beta} V_\beta \tlag{David.5} \eeq
We have for small velocities that
\beq U_\alpha = \lambda_{\alpha\beta} (\mathbf{X}) V_\beta + \Lambda_{\alpha\beta\gamma} (\mathbf{X}) V_\beta V_\gamma \tlag{David.6} \eeq
and so we find
\beq \gamma_{\alpha\beta} V_\beta = \lambda_{\alpha\beta}(\mathbf{X}) V_\beta + \Lambda_{\alpha\beta\gamma} (\mathbf{X}) V_\beta V_\gamma \tlag{David.7} \eeq
Written this way the term $\lambda_{\alpha\beta}(\mathbf{X})$ is just the friction tensor in the absence of any elastic effects. We can thus write
\beq \gamma_{\alpha\beta} = \lambda_{\alpha\beta} + \gamma_{2\alpha\beta} \tlag{David.8} \eeq
and we write
\beq \gamma_{2\alpha\beta} = \Gamma_{\alpha\beta\gamma} V_\gamma \tlag{David.9} \eeq
and
\beq \Gamma_{\alpha\beta\gamma} (\mathbf{X}) V_\beta V_\gamma = \Lambda_{\alpha\beta\gamma} (\mathbf{X}) V_\beta V_\gamma \tlag{David.10} \eeq
where we without loss of generality take $\Lambda_{\alpha\beta\gamma} = \Lambda_{\alpha\gamma\beta}$, which then gives
\beq \Gamma_{\alpha\beta\gamma} + \Gamma_{\alpha\gamma\beta} = 2 \Lambda_{\alpha\beta\gamma} \tlag{David.11} \eeq
We have to solve this system with the constraint that $\Gamma_{\alpha\beta\gamma} V_\gamma = \Gamma_{\beta\alpha\gamma} V_\gamma$. In Thomas' problem \tit{(see subsection \ref{ssc:Thomas})} we have
$$ \ddot{\Delta} + \xi \frac{\dot{\Delta}}{\Delta^{3/2}} + \frac{\kappa\xi}{4} \left[ 21 \frac{\dot{\Delta}^2}{\Delta^{9/2}} - \frac{(\dot\Theta - \dot{X}_G)^2}{\Delta^{7/2}} - \frac{15}{2} \frac{\ddot\Delta}{\Delta^{7/2}} \right] + \cos\alpha = 0 $$
$$ \ddot{X}_G + \frac{2\varepsilon \xi}{3} \frac{\dot{X}_G}{\sqrt\Delta} + \frac{\kappa \varepsilon \xi}{6} \left[ \frac{19}{4} \frac{\dot\Delta \dot{X}_G}{\Delta^{7/2}} - \frac{\dot\Delta \dot\Theta}{\Delta^{7/2}} + \frac{1}{2} \frac{\ddot\Theta - \ddot{X}_G}{\Delta^{5/2}} \right] - \sqrt{\frac{\varepsilon}{2}} \sin\alpha = 0 $$
\tit{where $\Delta$ refers to $z$ and $X_G$ refers to $x$. Note $\dot\Delta=-U_z$ and $\dot{X}_G=-U_x$, we write}
\beq U_z = \xi \frac{V_z}{Z^{3/2}} + \frac{21 \kappa \xi}{4} \frac{V_z^2}{Z^{9/2}} - \frac{\kappa \xi}{4} \frac{V_x^2}{Z^{7/2}}  \tlag{David.12} \eeq
\beq U_x = 2 \xi\veps \frac{V_x}{3Z^{1/2}} + \frac{19 \kappa \xi \veps}{24} \frac{V_z V_x}{Z^{7/2}} \tlag{David.13} \eeq
\textit{Note $\dot\Delta = V_z$ and $\dot{X}_G = V_x$, we could extract the relevant coefficients. But Attention! Here $\dot\Theta$ was assumed 0, and the second derivatives in first-order correlation had been ignored.} \\
Form this we find that
\beq \bgn
\sum_{\alpha\beta} \Lambda_{z\alpha\beta} V_\alpha V_\beta &= \frac{21 \kappa \xi}{4} \frac{V_z^2}{Z^{9/2}} - \frac{\kappa \xi}{4} \frac{V_x^2}{Z^{7/2}} \\
\sum_{\alpha\beta} \Lambda_{x\alpha\beta} V_\alpha V_\beta &= \frac{19 \kappa \xi \veps}{24} \frac{V_z V_x}{Z^{7/2}}
\end{align} \tlag{David.14} \eeq
This gives the set of equations
\beq \Gamma_{zzz} = \frac{21 \kappa \xi}{4 Z^{9/2}} \tlag{David.15} \eeq
\beq \Gamma_{zxx} = - \frac{\kappa \xi}{4Z^{7/2}} \tlag{David.16} \eeq

\beq \Gamma_{zxz} + \Gamma_{zzx} = 0 \tlag{David.17} \eeq
\beq \Gamma_{xzz} = 0 \tlag{David.18} \eeq
\beq \Gamma_{xxx} = 0 \tlag{David.19} \eeq
\beq \Gamma_{xxz} + \Gamma_{xzx} = \frac{19 \kappa \xi \veps}{24 Z^{7/2}} \tlag{David.20} \eeq
The symmetry $\Gamma_{\alpha\beta\gamma} = \Gamma_{\beta\alpha\gamma}$ now gives
\beq \Gamma_{xxz} = \frac{19 \kappa \xi \veps}{24 Z^{7/2}} - \Gamma_{xzx} = \frac{19 \kappa \xi \veps}{24 Z^{7/2}} - \Gamma_{zxx} = \frac{\kappa\xi}{Z^{7/2}} \left( \frac{19\veps}{24} + \frac{1}{4} \right) \tlag{David.21} \eeq
as well as
\beq \Gamma_{zxz} = \Gamma_{zzx} = 0 \tlag{David.22} \eeq
The Langevin equation corresponding to this is, using the It√¥ convention,
\beq \frac{dV_\alpha}{dt} = -U_\alpha - \pder[\phi(\mathbf{X})]{X_\alpha} + T \pder[\gamma_{\alpha\beta}]{V_\beta} + \eta_\alpha(t) \tlag{David.23} \eeq
which can be written as
\beq \frac{dV_\alpha}{dt} = -U_\alpha - \pder[\phi(\mathbf{X})]{X_\alpha} + T \Gamma_{\alpha\beta\beta} + \eta_\alpha(t) \tlag{David.24} \eeq
where we use the Einstein summation convention and the noise correlator is given by
\beq \llang \eta_\alpha (t) \eta_\beta(t^\prime) \rrang = 2T \gamma_{\alpha \beta} \delta(t-t^\prime) = 2T \left[ \lambda_{\alpha\beta}(\mathbf{X}) + \Gamma_{\alpha\beta\gamma}(\mathbf{X}) V_\gamma \right] \delta(t-t^\prime) \tlag{David.25} \eeq
Putting this together we find \tit{(from eq. \ref{David.24}) with all $\Gamma_{\alpha\beta\beta}$ only depending on $\Delta, X$.}
\beq \bgn
\frac{dV_z}{dt} &= -V^\prime(Z) - \xi \frac{V_z}{Z^{3/2}} - \frac{21\kappa\xi}{4}\frac{V_z^2}{Z^{9/2}} + \frac{\kappa \xi V_x^2}{4 Z^{7/2}} + T \left[ \frac{21 \kappa \xi}{4 Z^{9/2}} - \frac{\kappa \xi}{4 Z^{7/2}} \right] + \eta_z(t) \\
\frac{dV_x}{dt} &= -2\xi\veps \frac{V_x}{3 Z^{1/2}} - \frac{19 \kappa \xi \evps V_z V_x}{24 Z^{7/2}} + \eta_x(t) 
\end{align} \tlag{David.26} \eeq
